Update examples.logic to use Ecifcon and Ejudg

nola/examples/logic.v
@@ -7,263 +7,252 @@ From nola.examples Require Export nsynty.
 Import ProdNotation UpdwNotation WpwNotation iPropAppNotation ProphNotation
   LftNotation NsyntyNotation FunPRNotation DsemNotation.
 
-Implicit Type (Σ : gFunctors) (N : namespace) (dq : dfrac) (l : loc) (b : bool)
-  (α β : lft) (q : Qp) (X Y : nsynty).
+Implicit Type (Σ : gFunctors) (N : namespace) (TY : synty) (dq : dfrac)
+  (l : loc) (b : bool) (α β : lft) (q : Qp).
 
-(** ** Custom constructors *)
-
-(** [con_sel]: Selector *)
-Variant con_sel :=
-| (** Points-to token *) cifs_pointsto (l : loc) (dq : dfrac) (v : val)
-| (** Invariant *) cifs_inv (N : namespace)
-| (** Relaxed invariant *) cifs_inv' (N : namespace)
-| (** Non-prophetic borrower *) cifs_bor (α : lft)
-| (** Non-prophetic open borrower *) cifs_obor (α : lft) (q : Qp)
-| (** Non-prophetic lender *) cifs_lend (α : lft)
-| (** Prophetic borrower *) cifs_pbor {X} (α : lft) (x : X) (ξ : prvar X)
-| (** Prophetic open borrower *) cifs_pobor {X} (α : lft) (q : Qp) (ξ : prvar X)
-| (** Prophetic lender *) cifs_plend {X} (α : lft) (xπ : clair nsynty X).
-(** [con_idom]: Domain for inductive parts *)
-Definition con_idom (_ : con_sel) : Type := Empty_set.
-(** [con_cdom]: Domain for coinductive parts *)
-Definition con_cdom (s : con_sel) : Type := match s with
-  | cifs_pointsto _ _ _ => Empty_set
-  | cifs_inv _ | cifs_inv' _ | cifs_bor _ | cifs_obor _ _ | cifs_lend _ => unit
-  | @cifs_pbor X _ _ _ | @cifs_pobor X _ _ _ | @cifs_plend X _ _ => X
-  end.
-(** [con_data]: Data [oFunctor] *)
-Definition con_data (_ : con_sel) : oFunctor := unitO.
-(** [con]: Constructor structure *)
-Canonical con : cifcon := Cifcon con_sel con_idom con_cdom con_data _.
-
-(** ** [cif]: Formulas *)
-Notation cifOF := (cifOF con).
-Notation cif Σ := (cif con Σ).
-
-(** Construct [cif] *)
-Section cif.
-  Context {Σ}.
-  Implicit Type Px : cif Σ.
-  (** Points-to token *)
-  Definition cif_pointsto l dq v : cif Σ :=
-    cif_custom (cifs_pointsto l dq v) nullary nullary ().
-  (** Invariant *)
-  Definition cif_inv N Px : cif Σ :=
-    cif_custom (cifs_inv N) nullary (unary Px) ().
-  (** Relaxed invariant *)
-  Definition cif_inv' N Px : cif Σ :=
-    cif_custom (cifs_inv' N) nullary (unary Px) ().
-  (** Non-prophetic borrower *)
-  Definition cif_bor α Px : cif Σ :=
-    cif_custom (cifs_bor α) nullary (unary Px) ().
-  (** Non-prophetic open borrower *)
-  Definition cif_obor α q Px : cif Σ :=
-    cif_custom (cifs_obor α q) nullary (unary Px) ().
-  (** Non-prophetic lender *)
-  Definition cif_lend α Px : cif Σ :=
-    cif_custom (cifs_lend α) nullary (unary Px) ().
-  (** Prophetic borrower *)
-  Definition cif_pbor {X} α x ξ (Φx : X -pr> cif Σ) : cif Σ :=
-    cif_custom (@cifs_pbor X α x ξ) nullary Φx ().
-  (** Prophetic open borrower *)
-  Definition cif_pobor {X} α q ξ (Φx : X -pr> cif Σ) : cif Σ :=
-    cif_custom (@cifs_pobor X α q ξ) nullary Φx ().
-  (** Prophetic lender *)
-  Definition cif_plend {X} α xπ (Φx : X -pr> cif Σ) : cif Σ :=
-    cif_custom (@cifs_plend X α xπ) nullary Φx ().
-
-  (** The custom constructors are productive *)
-  #[export] Instance cif_inv_productive {N} : Productive (cif_inv N).
-  Proof.
-    move=> n ???. apply cif_custom_preserv_productive=>//. by destruct n=> >.
-  Qed.
-  #[export] Instance cif_inv'_productive  {N} : Productive (cif_inv' N).
-  Proof.
-    move=> n ???. apply cif_custom_preserv_productive=>//. by destruct n=> >.
-  Qed.
-  #[export] Instance cif_bor_productive {α} : Productive (cif_bor α).
-  Proof.
-    move=> n ???. apply cif_custom_preserv_productive=>//. by destruct n=> >.
-  Qed.
-  #[export] Instance cif_obor_productive {α q} : Productive (cif_obor α q).
-  Proof.
-    move=> n ???. apply cif_custom_preserv_productive=>//. by destruct n=> >.
-  Qed.
-  #[export] Instance cif_lend_productive {α} : Productive (cif_lend α).
-  Proof.
-    move=> n ???. apply cif_custom_preserv_productive=>//. by destruct n=> >.
-  Qed.
-  #[export] Instance cif_pbor_productive {X α x ξ} :
-    Productive (@cif_pbor X α x ξ).
-  Proof. solve_proper. Qed.
-  #[export] Instance cif_pobor_productive {X α q ξ} :
-    Productive (@cif_pobor X α q ξ).
-  Proof. solve_proper. Qed.
-  #[export] Instance cif_plend_productive {X α xπ} :
-    Productive (@cif_plend X α xπ).
-  Proof. solve_proper. Qed.
-
-  (** The custom constructors are non-expansive *)
+(** ** Invariant *)
+(** [invCC]: Constructor *)
+Definition invCC : cifcon :=
+  Cifcon namespace (λ _, Empty_set) (λ _, unit) (λ _, unitO) _.
+(** [InvCon]: [invCC] registered *)
+Notation InvCon CON := (Ecifcon invCC CON).
+Section cif_inv.
+  Context `{!InvCon CON} {Σ}.
+  (** [cif_inv]: Formula *)
+  Definition cif_inv N (Px : cif CON Σ) : cif CON Σ :=
+    cif_ecustom invCC N nullary (unary Px) ().
+  (** [cif_inv] is non-expansive *)
   #[export] Instance cif_inv_ne {N} : NonExpansive (cif_inv N).
-  Proof. solve_proper. Qed.
+  Proof. move=> ????. apply cif_ecustom_ne; solve_proper. Qed.
   #[export] Instance cif_inv_proper {N} : Proper ((≡) ==> (≡)) (cif_inv N).
   Proof. apply ne_proper, _. Qed.
-  #[export] Instance cif_inv'_ne {N} : NonExpansive (cif_inv' N).
-  Proof. solve_proper. Qed.
-  #[export] Instance cif_inv'_proper {N} : Proper ((≡) ==> (≡)) (cif_inv' N).
-  Proof. apply ne_proper, _. Qed.
+  (** [cif_inv] is productive *)
+  #[export] Instance cif_inv_productive {N} : Productive (cif_inv N).
+  Proof.
+    move=> ????. apply cif_ecustom_preserv_productive=>//.
+    by apply fun_proeq_later.
+  Qed.
+  Context `{!inv'GS (cifOF CON) Σ}.
+  (** Semantics of [invCC] *)
+  #[export] Program Instance inv_sem_ecifcon {JUDG}
+    : SemEcifcon JUDG invCC CON Σ :=
+    SEM_ECIFCON (λ _ N _ Φx _, inv_tok N (Φx ())) _.
+  Next Obligation. move=>/= ?????????? eqv ???. f_equiv. apply eqv. Qed.
+End cif_inv.
+(** [invCC] semantics registered *)
+Notation InvSem JUDG CON Σ := (EsemEcifcon JUDG invCC CON Σ).
+
+(** ** Borrow *)
+(** [borCC]: Constructor *)
+Definition borCC :=
+  Cifcon lft (λ _, Empty_set) (λ _, unit) (λ _, unitO) _.
+(** [BorCon]: [borCC] registered *)
+Notation BorCon CON := (Ecifcon borCC CON).
+Section cif_bor.
+  Context `{!BorCon CON} {Σ}.
+  (** [cif_bor]: Formula *)
+  Definition cif_bor α (Px : cif CON Σ) : cif CON Σ :=
+    cif_ecustom borCC α nullary (unary Px) ().
+  (** [cif_bor] is non-expansive *)
   #[export] Instance cif_bor_ne {α} : NonExpansive (cif_bor α).
-  Proof. solve_proper. Qed.
+  Proof. move=> ????. apply cif_ecustom_ne; solve_proper. Qed.
   #[export] Instance cif_bor_proper {α} : Proper ((≡) ==> (≡)) (cif_bor α).
   Proof. apply ne_proper, _. Qed.
-  #[export] Instance cif_obor_ne {α q} : NonExpansive (cif_obor α q).
-  Proof. solve_proper. Qed.
-  #[export] Instance cif_obor_proper {α q} :
-    Proper ((≡) ==> (≡)) (cif_obor α q).
-  Proof. apply ne_proper, _. Qed.
-  #[export] Instance cif_lend_ne {α} : NonExpansive (cif_lend α).
-  Proof. solve_proper. Qed.
-  #[export] Instance cif_lend_proper {α} : Proper ((≡) ==> (≡)) (cif_lend α).
-  Proof. apply ne_proper, _. Qed.
+  (** [cif_bor] is productive *)
+  #[export] Instance cif_bor_productive {α} : Productive (cif_bor α).
+  Proof.
+    move=> ????. apply cif_ecustom_preserv_productive=>//.
+    by apply fun_proeq_later.
+  Qed.
+  Context `{!pborrowGS TY (cifOF CON) Σ}.
+  (** Semantics of [borCC] *)
+  #[export] Program Instance bor_sem_ecifcon {JUDG}
+    : SemEcifcon JUDG borCC CON Σ :=
+    SEM_ECIFCON (λ _ α _ Φx _, nbor_tok α (Φx ())) _.
+  Next Obligation. move=>/= ?????????? eqv ???. f_equiv. apply eqv. Qed.
+End cif_bor.
+(** [borCC] semantics registered *)
+Notation BorSem JUDG CON Σ := (EsemEcifcon JUDG borCC CON Σ).
+
+(** ** Prophetic borrow *)
+(** [pborCC]: Constructor *)
+Definition pborCC TY :=
+  Cifcon (lft *' TY) (λ _, Empty_set) (λ '(_, X)', X)
+    (λ '(_, X)', leibnizO (X *' prvar X)) _.
+(** [PborCon]: [pborCC] registered *)
+Notation PborCon TY CON := (Ecifcon (pborCC TY) CON).
+Section cif_pbor.
+  Context `{!PborCon TY CON} {Σ}.
+  Implicit Type X : TY.
+  (** [cif_pbor]: Formula *)
+  Definition cif_pbor {X} α (x : X) (ξ : prvar X) (Φx : X -pr> cif CON Σ)
+    : cif CON Σ :=
+    cif_ecustom (pborCC TY) (α, X)' nullary Φx (x, ξ)'.
+  (** [cif_pbor] is non-expansive *)
   #[export] Instance cif_pbor_ne {X α x ξ} : NonExpansive (@cif_pbor X α x ξ).
   Proof. solve_proper. Qed.
   #[export] Instance cif_pbor_proper {X α x ξ} :
     Proper ((≡) ==> (≡)) (@cif_pbor X α x ξ).
   Proof. apply ne_proper, _. Qed.
-  #[export] Instance cif_pobor_ne {X α q ξ} : NonExpansive (@cif_pobor X α q ξ).
+  (** [cif_pbor] is productive *)
+  #[export] Instance cif_pbor_productive {X α x ξ} :
+    Productive (@cif_pbor X α x ξ).
   Proof. solve_proper. Qed.
-  #[export] Instance cif_pobor_proper {X α q ξ} :
-    Proper ((≡) ==> (≡)) (@cif_pobor X α q ξ).
-  Proof. apply ne_proper, _. Qed.
-  #[export] Instance cif_plend_ne {X α xπ} : NonExpansive (@cif_plend X α xπ).
+  Context `{!pborrowGS TY (cifOF CON) Σ}.
+  (** Semantics of [pborCC] *)
+  #[export] Program Instance pbor_sem_ecifcon {JUDG}
+    : SemEcifcon JUDG (pborCC TY) CON Σ :=
+    SEM_ECIFCON (λ _ '(α, X)' _ Φx '(x, ξ)', pbor_tok α x ξ Φx) _.
+  Next Obligation. move=>/= ????????????? /leibniz_equiv_iff. solve_proper. Qed.
+End cif_pbor.
+(** [pborCC] semantics registered *)
+Notation PborSem TY JUDG CON Σ := (EsemEcifcon JUDG (pborCC TY) CON Σ).
+
+(** ** Judgment *)
+Definition iff_judgty (FM : ofe) : ofe := (FM * FM)%type.
+Notation IffJudg FM JUDG := (Ejudg (iff_judgty FM) JUDG).
+Section iff_judg.
+  Context `{iff_judg : !IffJudg FM JUDG}.
+  Definition jiff (Px Qx : FM) : JUDG := iff_judg (Px, Qx).
+  #[export] Instance jiff_ne : NonExpansive2 jiff.
   Proof. solve_proper. Qed.
-  #[export] Instance cif_plend_proper {X α xπ} :
-    Proper ((≡) ==> (≡)) (@cif_plend X α xπ).
+
+  Context `{!Dsem JUDG FM (iProp Σ)}.
+  (** ** [iff_judg_sem]: Semantics of [iff_judgty] *)
+  Definition iff_judg_sem δ (PQx : iff_judgty FM) : iProp Σ :=
+    □ (⟦ PQx.1 ⟧(δ) ∗-∗ ⟦ PQx.2 ⟧(δ)).
+  (** [iff_judg_sem] is non-expansive *)
+  #[export] Instance iff_judg_sem_ne `{!NonExpansive δ} :
+    NonExpansive (iff_judg_sem δ).
+  Proof. solve_proper. Qed.
+  (** [Dsem] over [iff_judgty] *)
+  #[export] Instance iff_judg_dsem
+    : Dsem JUDG (iff_judgty FM) (iProp Σ) := DSEM iff_judg_sem _.
+End iff_judg.
+(** ** [IffJsem]: Judgment semantics for [iff] *)
+Notation IffJsem FM Σ JUDG := (Ejsem (iff_judgty FM) JUDG (iProp Σ)).
+
+Section iff_judg.
+  Context `{!Jsem JUDG (iProp Σ), !Dsem JUDG FM (iProp Σ), !IffJudg FM JUDG,
+    !IffJsem FM Σ JUDG}.
+
+  (** Derivability of [jiff] is persistent *)
+  #[export] Instance Deriv_jiff_persistent `{!Deriv (JUDG:=JUDG) ih δ} {Px Qx} :
+    Persistent (δ (jiff Px Qx)).
+  Proof. apply: Deriv_persistent=> ????. rewrite sem_ejudg. exact _. Qed.
+End iff_judg.
+
+(** ** Relaxed invariant *)
+(** [inv'CC]: Constructor *)
+Definition inv'CC : cifcon :=
+  Cifcon (namespace *' unit) (λ _, Empty_set) (λ _, unit) (λ _, unitO) _.
+(** [Inv'Con]: [inv'CC] registered *)
+Notation Inv'Con CON := (Ecifcon inv'CC CON).
+Section cif_inv'.
+  Context `{!Inv'Con CON} {Σ}.
+  (** [cif_inv']: Formula *)
+  Definition cif_inv' N (Px : cif CON Σ) : cif CON Σ :=
+    cif_ecustom inv'CC (N, ())' nullary (unary Px) ().
+  (** [cif_inv'] is non-expansive *)
+  #[export] Instance cif_inv'_ne {N} : NonExpansive (cif_inv' N).
+  Proof. move=> ????. apply cif_ecustom_ne; solve_proper. Qed.
+  #[export] Instance cif_inv'_proper {N} : Proper ((≡) ==> (≡)) (cif_inv' N).
   Proof. apply ne_proper, _. Qed.
-End cif.
-Notation "l ↦ dq v" := (cif_pointsto l dq v)
-  (at level 20, dq custom dfrac at level 1, format "l  ↦ dq  v") : cif_scope.
+  (** [cif_inv'] is productive *)
+  #[export] Instance cif_inv'_productive {N} : Productive (cif_inv' N).
+  Proof.
+    move=> ????. apply cif_ecustom_preserv_productive=>//.
+    by apply fun_proeq_later.
+  Qed.
 
-(** ** [judg]: Judgment *)
-Definition judg Σ : ofe := (cif Σ * cif Σ)%type.
-
-Section sem.
-  Context `{!inv'GS cifOF Σ, !pborrowGS nsynty cifOF Σ, !heapGS_gen hlc Σ}.
-  Implicit Type (δ : judg Σ → iProp Σ) (Px : cif Σ).
-
-  (** Relaxed invariant *)
-  Definition inv' δ N Px : iProp Σ := ∃ Qx, δ (Px, Qx) ∗ inv_tok N Qx.
+  Context `{!inv'GS (cifOF CON) Σ, !IffJudg (cifO CON Σ) JUDG}.
+  (** [inv']: Relaxed invariant *)
+  Definition inv' δ N Px : iProp Σ := ∃ Qx, δ (jiff Px Qx) ∗ inv_tok N Qx.
   (** [inv'] is non-expansive *)
   #[export] Instance inv'_ne `{!NonExpansive δ} {N} : NonExpansive (inv' δ N).
   Proof. solve_proper. Qed.
   #[export] Instance inv'_proper `{!NonExpansive δ} {N} :
     Proper ((≡) ==> (⊣⊢)) (inv' δ N).
   Proof. apply ne_proper, _. Qed.
-
-  (** ** Constructor semantics *)
-  Definition con_sem δ s : (con_idom s -d> iProp Σ) →
-    (con_cdom s -d> cif Σ) → con_data s $oi Σ → iProp Σ :=
-    match s with
-    | cifs_pointsto l dq v => λ _ _ _, l ↦{dq} v
-    | cifs_inv N => λ _ Pxs _, inv_tok N (Pxs ())
-    | cifs_inv' N => λ _ Pxs _, inv' δ N (Pxs ())
-    | cifs_bor α => λ _ Pxs _, nbor_tok α (Pxs ())
-    | cifs_obor α q => λ _ Pxs _, nobor_tok α q (Pxs ())
-    | cifs_lend α => λ _ Pxs _, nlend_tok α (Pxs ())
-    | cifs_pbor α x ξ => λ _ Φx _, pbor_tok α x ξ Φx
-    | cifs_pobor α q ξ => λ _ Φx _, pobor_tok α q ξ Φx
-    | cifs_plend α xπ => λ _ Φx _, plend_tok α xπ Φx
-    end%I.
-  #[export] Instance con_sem_ne `{!NonExpansive δ} {s} :
-    NonExpansive3 (con_sem δ s).
-  Proof.
-    move=> ?????? eqv ??? /=. destruct s=>//=; repeat f_equiv; apply eqv.
-  Qed.
-  #[export] Instance con_sem_cifcon : SemCifcon (judg Σ) con Σ :=
-    SEM_CIFCON con_sem _.
-
-  (** Judgment semantics *)
-  Definition judg_sem δ (J : judg Σ) : iProp Σ := □ (⟦ J.1 ⟧(δ) ∗-∗ ⟦ J.2 ⟧(δ)).
-  #[export] Instance judg_sem_ne `{!NonExpansive δ} : NonExpansive (judg_sem δ).
-  Proof. solve_proper. Qed.
-  #[export] Instance judg_jsem : Jsem (judg Σ) (iProp Σ) :=
-    DSEM judg_sem _.
-
-  (** Simplify [to_cit (of_cit Px)] *)
-  Lemma sem_to_of_cit `{!NonExpansive δ} {Px} :
-    cif_sem δ (to_cit (of_cit Px)) ⊣⊢ ⟦ Px ⟧(δ).
-  Proof. by rewrite to_of_cit. Qed.
-End sem.
-
+  (** Semantics of [invCC] *)
+  #[export] Program Instance inv'_sem_ecifcon
+    : SemEcifcon JUDG inv'CC CON Σ :=
+    SEM_ECIFCON (λ δ '(N, _)' _ Φx _, inv' δ N (Φx ())) _.
+  Next Obligation. solve_proper. Qed.
+End cif_inv'.
+(** [inv'CC] semantics registered *)
+Notation Inv'Sem JUDG CON Σ := (EsemEcifcon JUDG inv'CC CON Σ).
+(** Notation *)
 Notation invd := (inv' der).
 
 Section verify.
-  Context `{!inv'GS cifOF Σ, !pborrowGS nsynty cifOF Σ, !heapGS_gen hlc Σ}.
-  Implicit Type (Px Qx : cif Σ) (Φx Ψx : loc → cif Σ).
+  Context `{!heapGS_gen hlc Σ, !SemCifcon JUDG CON Σ, !Jsem JUDG (iProp Σ)}.
+  Context `{!inv'GS (cifOF CON) Σ, !InvCon CON, !InvSem JUDG CON Σ}.
+  Implicit Type (Px Qx : cif CON Σ) (Φx Ψx : loc → cif CON Σ).
 
   (** ** Linked list *)
 
-  (** [ilist]: Formula for a list *)
-  Definition ilist_gen N (Φx : loc -pr> cif Σ)
-    (Ilist : loc -pr> cif Σ) : loc -pr> cif Σ :=
-    λ l, (cif_inv N (Φx l) ∗ cif_inv N (∃ l', (l +ₗ 1) ↦ #l' ∗ Ilist l'))%cif.
+  (** [cif_ilist]: Formula for a list *)
+  Definition cif_ilist_gen N (Φx : loc -pr> cif CON Σ)
+    (Ilist : loc -pr> cif CON Σ) : loc -pr> cif CON Σ :=
+    λ l, (cif_inv N (Φx l) ∗ cif_inv N (∃ l', ▷ (l +ₗ 1) ↦ #l' ∗ Ilist l'))%cif.
   #[export] Instance ilist_gen_productive {n N} :
-    Proper (proeq_later n ==> proeq_later n ==> proeq n) (ilist_gen N).
+    Proper (proeq_later n ==> proeq_later n ==> proeq n) (cif_ilist_gen N).
   Proof.
-    move=>/= ?? eq ?? eq' ?. unfold ilist_gen.
+    move=>/= ?? eq ?? eq' ?. unfold cif_ilist_gen.
     f_equiv; apply cif_inv_productive; (destruct n as [|n]; [done|]);
       [apply eq|]=>/=.
     f_equiv=> ?. by f_equiv.
   Qed.
-  #[export] Instance ilist_gen_productive' {N Φx} :
-    Productive (ilist_gen N Φx).
+  #[export] Instance cif_ilist_gen_productive' {N Φx} :
+    Productive (cif_ilist_gen N Φx).
   Proof. move=> ?. by apply ilist_gen_productive. Qed.
-  Definition ilist' N (Φx : loc -pr> cif Σ) : loc -pr> cif Σ :=
-    profix (ilist_gen N Φx).
-  Definition ilist N (Φx : loc -pr> cif Σ) : loc -pr> cif Σ :=
-    ilist_gen N Φx (ilist' N Φx).
-  (** Unfold [ilist'] *)
-  Lemma ilist'_unfold {N Φx l} : ilist' N Φx l ≡ ilist N Φx l.
-  Proof. by rewrite /ilist' (profix_unfold (f:=ilist_gen _ _) l). Qed.
+  Definition cif_ilist N (Φx : loc -pr> cif CON Σ) : loc -pr> cif CON Σ :=
+    profix (cif_ilist_gen N Φx).
+  (** Unfold [cif_ilist] *)
+  Lemma cif_ilist_unfold {N Φx l} :
+    cif_ilist N Φx l ≡ cif_ilist_gen N Φx (cif_ilist N Φx) l.
+  Proof. by rewrite /cif_ilist (profix_unfold (f:=cif_ilist_gen _ _) l). Qed.
+  (** Semantics *)
+  Definition ilist N Φx l : iProp Σ := inv_tok N (Φx l) ∗
+    inv_tok N (∃ l', ▷ (l +ₗ 1) ↦ #l' ∗ cif_ilist N Φx l')%cif.
+  (** Unfold semantics over [cif_ilist] *)
+  Lemma sem_ilist `{!NonExpansive δ} {N Φx l} :
+    cif_sem δ (cif_ilist N Φx l) ⊣⊢ ilist N Φx l.
+  Proof. by rewrite cif_ilist_unfold /= !sem_ecustom /=. Qed.
 
-  (** [ilist'] is productive *)
-  #[export] Instance ilist'_productive {N} : Productive (ilist' N).
+  (** [cif_ilist] is productive *)
+  #[export] Instance cif_ilist_productive {N} : Productive (cif_ilist N).
   Proof. move=> ????. apply profix_preserv=> ?. by f_equiv. Qed.
-  #[export] Instance ilist_productive {N} : Productive (ilist N).
-  Proof.
-    move=> n ?? eq. apply ilist_gen_productive=>//. destruct n as [|n]=>//= ?.
-    apply ilist'_productive. move: eq. apply proeq_later_anti. lia.
-  Qed.
 
-  (** [ilist_gen] is non-expansive *)
-  #[export] Instance ilist_gen_ne {N} : NonExpansive2 (ilist_gen N).
-  Proof. unfold ilist_gen=> ????????. (do 3 f_equiv=>//)=> ?. by f_equiv. Qed.
-  #[export] Instance ilist_gen_proper {N} :
-    Proper ((≡) ==> (≡) ==> (≡)) (ilist_gen N).
+  (** [cif_ilist_gen] is non-expansive *)
+  #[export] Instance cif_ilist_gen_ne {N} : NonExpansive2 (cif_ilist_gen N).
+  Proof.
+    unfold cif_ilist_gen=> ????????. (do 3 f_equiv=>//)=> ?. by f_equiv.
+  Qed.
+  #[export] Instance cif_ilist_gen_proper {N} :
+    Proper ((≡) ==> (≡) ==> (≡)) (cif_ilist_gen N).
   Proof. apply ne_proper_2, _. Qed.
-  (** [ilist'] is non-expansive *)
-  #[export] Instance ilist'_ne {N} : NonExpansive (ilist' N).
+  (** [cif_ilist] is non-expansive *)
+  #[export] Instance cif_ilist_ne {N} : NonExpansive (cif_ilist N).
   Proof. move=> ????. apply profix_ne=> ???. by f_equiv. Qed.
-  #[export] Instance ilist'_proper {N} : Proper ((≡) ==> (≡)) (ilist' N).
-  Proof. apply ne_proper, _. Qed.
-  #[export] Instance ilist_ne {N} : NonExpansive (ilist N).
-  Proof. unfold ilist=> ????. f_equiv=>//. by f_equiv. Qed.
-  #[export] Instance ilist_proper {N} : Proper ((≡) ==> (≡)) (ilist N).
+  #[export] Instance cif_ilist_proper {N} :
+    Proper ((≡) ==> (≡)) (cif_ilist N).
   Proof. apply ne_proper, _. Qed.
 
   (** Access the tail of a list *)
   Definition tail_ilist : val := λ: "l", !("l" +ₗ #1).
   Lemma twp_tail_list {N E Φx l} : ↑N ⊆ E →
-    [[{ ⟦ ilist N Φx l ⟧ }]][inv_wsat ⟦⟧]
+    [[{ ilist N Φx l }]][inv_wsat ⟦⟧]
       tail_ilist #l @ E
-    [[{ l', RET #l'; ⟦ ilist N Φx l' ⟧ }]].
+    [[{ l', RET #l'; ilist N Φx l' }]].
   Proof.
-    iIntros (? Ψ) "/= #[_ itl] →Ψ". wp_rec. wp_pure.
-    iMod (inv_tok_acc with "itl") as "[↦ltl cl]"; [done|].
-    rewrite sem_to_of_cit /=. iDestruct "↦ltl" as (?) "[↦l' ltl]".
-    rewrite ilist'_unfold /=. iDestruct "ltl" as "#ltl". wp_load. iModIntro.
-    iMod ("cl" with "[$↦l']") as "_"; [by rewrite ilist'_unfold|]. iModIntro.
-    iApply ("→Ψ" with "ltl").
+    iIntros (? Ψ) "/= [_ #itl] →Ψ". wp_rec. wp_pure.
+    iMod (inv_tok_acc with "itl") as "/=[(%l' & >↦l' & ltl) cl]"; [done|].
+    rewrite sem_ilist. iDestruct "ltl" as "#ltl".
+    wp_load. iModIntro. iMod ("cl" with "[$↦l']") as "_".
+    { by rewrite sem_ilist. }
+    iModIntro. iApply ("→Ψ" with "ltl").
   Qed.
 
   (** Iterate over a list *)
@@ -273,7 +262,7 @@ Section verify.
   Lemma twp_iter_list {N E Φx c l} {f : val} {n : nat} : ↑N ⊆ E →
     (∀ l', [[{ inv_tok N (Φx l') }]][inv_wsat ⟦⟧] f #l' @ E
       [[{ RET #(); True }]]) -∗
-    [[{ c ↦ #n ∗ ⟦ ilist N Φx l ⟧ }]][inv_wsat ⟦⟧]
+    [[{ c ↦ #n ∗ ilist N Φx l }]][inv_wsat ⟦⟧]
       iter_ilist f #c #l @ E
     [[{ RET #(); c ↦ #0 }]].
   Proof.
@@ -281,7 +270,7 @@ Section verify.
     iInduction n as [|m] "IH" forall (l) "l".
     { wp_rec. wp_load. wp_pures. by iApply "→Ψ". }
     wp_rec. wp_load. wp_pures. wp_apply "f".
-    { rewrite to_of_cit. iDestruct "l" as "[$ _]". }
+    { iDestruct "l" as "[$ _]". }
     iIntros "_". wp_load. wp_store. have -> : (S m - 1)%Z = m by lia.
     wp_apply twp_tail_list; [done..|]. iIntros (l') "#ltl".
     iApply ("IH" with "c↦ →Ψ ltl").
@@ -291,7 +280,7 @@ Section verify.
   Lemma twp_fork_iter_list {N E Φx c' c l} {f : val} {m n : nat} : ↑N ⊆ E →
     (∀ l', [[{ inv_tok N (Φx l') }]][inv_wsat ⟦⟧] f #l' @ E
       [[{ RET #(); True }]]) -∗
-    [[{ c' ↦ #m ∗ c ↦ #n ∗ ⟦ ilist N Φx l ⟧ }]][inv_wsat ⟦⟧]
+    [[{ c' ↦ #m ∗ c ↦ #n ∗ ilist N Φx l }]][inv_wsat ⟦⟧]
       Fork (iter_ilist f #c' #l);; iter_ilist f #c #l @ E
     [[{ RET #(); c ↦ #0 }]].
   Proof.
@@ -310,7 +299,7 @@ Section verify.
   Lemma twp_forks_iter_list {N E Φx k l} {f : val} {n : nat} :
     (∀ l', [[{ inv_tok N (Φx l') }]][inv_wsat ⟦⟧] f #l'
       [[{ RET #(); True }]]) -∗
-    [[{ k ↦ #n ∗ ⟦ ilist N Φx l ⟧ }]][inv_wsat ⟦⟧]
+    [[{ k ↦ #n ∗ ilist N Φx l }]][inv_wsat ⟦⟧]
       forks_iter_list f #k #l @ E
     [[{ RET #(); k ↦ #0 }]].
   Proof.
@@ -325,7 +314,7 @@ Section verify.
   Lemma twp_nd_forks_iter_list {N E Φx l} {f : val} :
     (∀ l', [[{ inv_tok N (Φx l') }]][inv_wsat ⟦⟧] f #l'
       [[{ RET #(); True }]]) -∗
-    [[{ ⟦ ilist N Φx l ⟧ }]][inv_wsat ⟦⟧]
+    [[{ ilist N Φx l }]][inv_wsat ⟦⟧]
       let: "k" := ref Ndnat in forks_iter_list f "k" #l @ E
     [[{ RET #(); True }]].
   Proof.
@@ -346,32 +335,40 @@ Section verify.
   (** Release the lock on the mutex *)
   Definition release_mutex : val := λ: "l", "l" <- #false.
 
+  Context `{!pborrowGS nsynty (cifOF CON) Σ, !BorCon CON, !BorSem JUDG CON Σ}.
+
   (** ** On borrows *)
 
   (** Dereference a nested mutable reference *)
   Lemma bor_bor_deref {α β l Φx q} :
-    [[{ β ⊑□ α ∗ q.[β] ∗ nbor_tok β (∃ l', l ↦ #l' ∗ cif_bor α (Φx l'))%cif }]]
+    [[{ β ⊑□ α ∗ q.[β] ∗
+      nbor_tok β (∃ l', ▷ l ↦ #l' ∗ cif_bor α (Φx l'))%cif }]]
       [pborrow_wsat bupd ⟦⟧]
       !#l
     [[{ l', RET #l'; q.[β] ∗ nbor_tok β (Φx l') }]].
   Proof.
     iIntros (Ψ) "(#⊑ & [β β'] & b) →Ψ".
-    iMod (nbor_tok_open (M:=bupd) with "β b") as "/=[o [%l'[↦ b']]]".
+    iMod (nbor_tok_open (M:=bupd) with "β b") as "/=[o [%l'[>↦ b']]]".
     iApply twpw_fupdw_nonval; [done|]. wp_load. iModIntro.
     iMod (lft_sincl_live_acc with "⊑ β'") as (?) "[α →β']".
+    rewrite sem_ecustom /=.
     iMod (nbor_tok_reborrow (M:=bupd) with "⊑ α b'") as "(α & →b' & b')".
     iDestruct ("→β'" with "α") as "β'".
     iMod (nobor_tok_subdiv (M:=bupd) [] with "[] o [] [↦ →b']") as "[β _]"=>/=.
     { iApply lft_sincl_refl. } { done. }
-    { iIntros "† _". iModIntro. iExists _. iFrame "↦". by iApply "→b'". }
-    iModIntro. iApply "→Ψ". rewrite to_of_cit. iFrame.
+    { iIntros "† _". iModIntro. iExists _. iFrame "↦". rewrite sem_ecustom /=.
+      by iApply "→b'". }
+    iModIntro. iApply "→Ψ". iFrame.
   Qed.
+
+  Context `{!PborCon nsynty CON, !PborSem nsynty JUDG CON Σ}.
+  Implicit Type X : nsynty.
 
   (** Dereference a nested prophetic mutable reference *)
   Lemma pbor_pbor_deref {X η ξ α β l Φxx q} {x : X} :
     [[{ β ⊑□ α ∗ q.[β] ∗
         pbor_tok β ((x, ξ)' : _ *'ₛ prvarₛ _) η
-          (λ '(x', ξ')', ∃ l', l ↦ #l' ∗ cif_pbor α x' ξ' (Φxx l'))%cif }]]
+          (λ '(x', ξ')', ∃ l', ▷ l ↦ #l' ∗ cif_pbor α x' ξ' (Φxx l'))%cif }]]
       [pborrow_wsat bupd ⟦⟧]
       !#l
     [[{ l', RET #l';
@@ -379,43 +376,41 @@ Section verify.
           ⟨π, π η = (π ξ', ξ)'⟩ ∗ pbor_tok β x ξ' (Φxx l') }]].
   Proof.
     iIntros (Ψ) "(#⊑ & [β β'] & b) →Ψ".
-    iMod (pbor_tok_open (M:=bupd) with "β b") as "/=[o[%l'[↦ b']]]".
+    iMod (pbor_tok_open (M:=bupd) with "β b") as "/=[o[%l'[>↦ b']]]".
     iApply twpw_fupdw_nonval; [done|]. wp_load. iModIntro.
     iMod (lft_sincl_live_acc with "⊑ β'") as (?) "[α →β']".
+    rewrite sem_ecustom /=.
     iMod (pobor_pbor_tok_reborrow (TY:=nsynty) (M:=bupd)
       (λ _, (_,_)' : _ *'ₛ _) with "⊑ o α b' [↦]") as (?) "(β & α & obs & b)".
-    { iIntros "/=% _ ? !>". iExists _. iFrame. }
-    iModIntro. iApply "→Ψ". iDestruct ("→β'" with "α") as "$". iFrame "β".
-    iExists _. iFrame "obs". iClear "⊑". iStopProof. apply bi.equiv_entails.
-    f_equiv=> ?. by rewrite to_of_cit.
+    { iIntros "/=% _ ? !>". iExists _. iFrame "↦". by rewrite sem_ecustom /=. }
+    iModIntro. iApply "→Ψ". iDestruct ("→β'" with "α") as "$". iFrame.
   Qed.
 
   (** Load from an immutable shared borrow *)
   Lemma imbor_load {l α q} {n : Z} :
-    [[{ q.[α] ∗ inv_tok nroot (cif_bor α (l ↦ #n)) }]]
+    [[{ q.[α] ∗ inv_tok nroot (cif_bor α (▷ l ↦ #n)) }]]
       [inv_wsat ⟦⟧ ∗ pborrow_wsat bupd ⟦⟧]
       !#l
     [[{ RET #n; q.[α] }]].
   Proof.
-    iIntros (Φ) "[α #i] →Φ".
-    iMod (inv_tok_acc with "i") as "/=[b cl]"; [done|].
-    iMod (nbor_tok_open (M:=bupd) with "α b") as "[o ↦]".
-    rewrite sem_to_of_cit /=. wp_load. iModIntro.
-    iMod (nobor_tok_close (M:=bupd) with "o [↦]") as "[α b]".
-    { by rewrite sem_to_of_cit. }
+    iIntros (Φ) "[α #i] →Φ". iMod (inv_tok_acc with "i") as "/=[b cl]"; [done|].
+    rewrite sem_ecustom /=.
+    iMod (nbor_tok_open (M:=bupd) with "α b") as "/=[o >↦]". wp_load. iModIntro.
+    iMod (nobor_tok_close (M:=bupd) with "o [↦]") as "[α b]"=>/=; [done|].
     iMod ("cl" with "b") as "_". iModIntro. by iApply "→Φ".
   Qed.
 
   (** Shared borrow of a mutex *)
-  Definition mutex_bor' α l Px :=
-    cif_bor α ((l ↦ #false ∗ cif_bor α Px) ∨ l ↦ #true).
-  Definition mutex_bor α l Px := inv_tok nroot (mutex_bor' α l Px).
-  Definition cif_mutex_bor α l Px := cif_inv nroot (mutex_bor' α l Px).
-  #[export] Instance mutex_bor'_productive {α l} :
-    Productive (mutex_bor' α l).
+  Definition cif_mutex_bor' α l Px :=
+    cif_bor α ((▷ l ↦ #false ∗ cif_bor α Px) ∨ ▷ l ↦ #true).
+  Definition mutex_bor α l Px := inv_tok nroot (cif_mutex_bor' α l Px).
+  Definition cif_mutex_bor α l Px := cif_inv nroot (cif_mutex_bor' α l Px).
+  (** [cif_mutex_bor'] is productive *)
+  #[export] Instance cif_mutex_bor'_productive {α l} :
+    Productive (cif_mutex_bor' α l).
   Proof.
-    unfold mutex_bor'=> n ?? eq. f_equiv. destruct n as [|n]=>//=. do 3 f_equiv.
-    move: eq. apply proeq_later_anti. lia.
+    unfold cif_mutex_bor'=> n ?? eq. f_equiv. destruct n as [|n]=>//=.
+    do 3 f_equiv. move: eq. apply proeq_later_anti. lia.
   Qed.
   #[export] Instance cif_mutex_bor_productive {α l} :
     Productive (cif_mutex_bor α l).
@@ -423,6 +418,18 @@ Section verify.
     unfold cif_mutex_bor=> n ?? eq. f_equiv. destruct n as [|n]=>//=. f_equiv.
     move: eq. apply proeq_later_anti. lia.
   Qed.
+  (** [cif_mutex_bor'] is non-expansive *)
+  #[export] Instance cif_mutex_bor'_ne {α l} :
+    NonExpansive (cif_mutex_bor' α l).
+  Proof. solve_proper. Qed.
+  #[export] Instance cif_mutex_bor'_proper {α l} :
+    Proper ((≡) ==> (≡)) (cif_mutex_bor' α l).
+  Proof. apply ne_proper, _. Qed.
+  #[export] Instance cif_mutex_bor_ne {α l} : NonExpansive (cif_mutex_bor α l).
+  Proof. solve_proper. Qed.
+  #[export] Instance cif_mutex_bor_proper {α l} :
+    Proper ((≡) ==> (≡)) (cif_mutex_bor α l).
+  Proof. apply ne_proper, _. Qed.
 
   (** Try to acquire a lock from a shared borrow over a mutex *)
   Lemma mutex_bor_try_acquire {α l Px q} :
@@ -431,15 +438,14 @@ Section verify.
     [[{ b, RET #b; (if b then nbor_tok α Px else True) ∗ q.[α] }]].
   Proof.
     iIntros (Φ) "[#m [α α']] →Φ". wp_lam. wp_bind (CmpXchg _ _ _).
-    iMod (inv_tok_acc with "m") as "/=[b cl]"; [done|].
+    iMod (inv_tok_acc with "m") as "/=[b cl]"; [done|]. rewrite sem_ecustom /=.
     iMod (nbor_tok_open (M:=bupd) with "α b") as "[o big]".
-    rewrite sem_to_of_cit /=.
-    iDestruct "big" as "[[↦ b']|↦]"; [wp_cmpxchg_suc|wp_cmpxchg_fail];
+    rewrite /= sem_ecustom.
+    iDestruct "big" as "[[>↦ b']|>↦]"; [wp_cmpxchg_suc|wp_cmpxchg_fail];
       iModIntro;
-      (iMod (nobor_tok_close (M:=bupd) with "o [↦]") as "[α b]";
-        [rewrite sem_to_of_cit /=; by iFrame|]);
-      iMod ("cl" with "b") as "_"; iModIntro; wp_pure; iApply "→Φ"; iFrame=>//.
-    by rewrite to_of_cit.
+      (iMod (nobor_tok_close (M:=bupd) with "o [↦]") as "[α b]"=>/=;
+        [by iFrame|]);
+      iMod ("cl" with "b") as "_"; iModIntro; wp_pure; iApply "→Φ"; by iFrame.
   Qed.
   (** [mutex_bor_try_acquire], repeatedly with a timeout *)
   Lemma mutex_bor_try_acquire_loop {α l Px q} {n : nat} :
@@ -465,58 +471,66 @@ Section verify.
   Proof.
     iIntros (Φ) "(#m & b' & α) →Φ". wp_lam.
     iMod (inv_tok_acc with "m") as "/=[b cl]"; [done|].
-    iMod (nbor_tok_open (M:=bupd) with "α b") as "[o big]".
-    rewrite sem_to_of_cit /=.
-    iAssert (∃ b, l ↦ #b)%I with "[big]" as (?) "↦".
+    rewrite sem_ecustom /=.
+    iMod (nbor_tok_open (M:=bupd) with "α b") as "[o big]"=>/=.
+    iAssert (∃ b, ▷ l ↦ #b)%I with "[big]" as (?) ">↦".
     { iDestruct "big" as "[[$ _]|$]". }
-    wp_store. iModIntro. rewrite to_of_cit.
-    iMod (nobor_tok_close (M:=bupd) with "o [b' ↦]") as "/=[α b]".
-    { rewrite /= to_of_cit. iLeft. iFrame. }
+    wp_store. iModIntro.
+    iMod (nobor_tok_close (M:=bupd) with "o [b' ↦]") as "[α b]"=>/=.
+    { iLeft. rewrite sem_ecustom /=. iFrame. }
     iMod ("cl" with "b") as "_". iModIntro. by iApply "→Φ".
   Qed.
 
   (** Create a shared borrow and a lender of a mutex *)
   Lemma mutex_bor_lend_new {α l Px b q} :
     l ↦ #b -∗ ⟦ Px ⟧ -∗ q.[α] =[inv_wsat ⟦⟧ ∗ pborrow_wsat bupd ⟦⟧]=∗
-      mutex_bor α l Px ∗ nlend_tok α (∃ b', l ↦ #b' ∗ Px)%cif ∗ q.[α].
+      mutex_bor α l Px ∗ nlend_tok α (∃ b', ▷ l ↦ #b' ∗ Px)%cif ∗ q.[α].
   Proof.
     iIntros "↦ Px α".
     iMod (nbor_nlend_tok_new (M:=bupd) with "[↦ Px]") as "[b $]"; [by iFrame|].
     iMod (nbor_tok_open (M:=bupd) with "α b") as "/=[o[%b'[↦ Px]]]".
-    iMod (nobor_tok_subdiv (FML:=cifOF) (M:=bupd)
-      [∃ b', l ↦ #b'; Px]%cif with "[] o [↦ Px] []")
+    iMod (nobor_tok_subdiv (FML:=cifOF CON) (M:=bupd)
+      [∃ b', ▷ l ↦ #b'; Px]%cif with "[] o [↦ Px] []")
       as "(α & _ & (b & b' & _))"=>/=.
     { iApply lft_sincl_refl. } { iSplitL "↦"; iFrame. }
     { by iIntros "_ [[% $][$ _]]". }
     iMod (nbor_tok_open (M:=bupd) with "α b") as "/=[o ↦]".
-    iMod (nobor_tok_subdiv (FML:=cifOF) (M:=bupd)
-      [(l ↦ #false ∗ cif_bor α Px) ∨ l ↦ #true]%cif with "[] o [↦ b'] []")
+    iMod (nobor_tok_subdiv (FML:=cifOF CON) (M:=bupd)
+      [(▷ l ↦ #false ∗ cif_bor α Px) ∨ ▷ l ↦ #true]%cif with "[] o [↦ b'] []")
       as "($ & _ & [b _])"=>/=. { iApply lft_sincl_refl. }
-    { iSplit; [|done]. rewrite to_of_cit.
+    { iSplit; [|done]. rewrite sem_ecustom /=.
       iDestruct "↦" as ([|]) "↦"; [|iLeft]; iFrame. }
     { by iIntros "_ [[[$ _]|$]_]". }
-    iMod (inv_tok_alloc with "[b]") as "$"=>//=. by rewrite to_of_cit.
+    iMod (inv_tok_alloc with "[b]") as "$"=>//=. by rewrite sem_ecustom.
   Qed.
 
   (** ** Linked list with a shared borrow over a mutex *)
 
-  (** [mblist]: Formula for a list with a shared borrow over a mutex *)
-  Definition mblist_gen α (Φx : loc -pr> cif Σ) (Mblist : loc -pr> cif Σ)
-    : loc -pr> cif Σ :=
-    λ l, cif_mutex_bor α l (Φx (l +ₗ 1) ∗ ∃ l', (l +ₗ 2) ↦ #l' ∗ Mblist l').
-  #[export] Instance mblist_gen_productive {α Φx} :
-    Productive (mblist_gen α Φx).
+  (** [cif_mblist]: Formula for a list with a shared borrow over a mutex *)
+  Definition cif_mblist_gen α (Φx : loc -pr> cif CON Σ)
+    (Mblist : loc -pr> cif CON Σ) : loc -pr> cif CON Σ :=
+    λ l, cif_mutex_bor α l (Φx (l +ₗ 1) ∗ ∃ l', ▷ (l +ₗ 2) ↦ #l' ∗ Mblist l').
+  #[export] Instance cif_mblist_gen_productive {α Φx} :
+    Productive (cif_mblist_gen α Φx).
   Proof.
-    move=>/= n ?? eq ?. unfold mblist_gen. apply cif_mutex_bor_productive.
+    move=>/= n ?? eq ?. unfold cif_mblist_gen. apply cif_mutex_bor_productive.
     destruct n as [|n]=>//=. (do 2 f_equiv)=> ?. f_equiv. apply eq.
   Qed.
-  Definition mblist' α Φx : loc → cif Σ := profix (mblist_gen α Φx).
-  Definition mblist α Φx : loc → cif Σ := mblist_gen α Φx (mblist' α Φx).
-  (** Unfold [mblist'] *)
-  Lemma mblist'_unfold {α Φx l} : mblist' α Φx l ≡ mblist α Φx l.
-  Proof. by rewrite /mblist' (profix_unfold (f:=mblist_gen _ _) l). Qed.
+  Definition cif_mblist α Φx : loc → cif CON Σ :=
+    profix (cif_mblist_gen α Φx).
+  (** Unfold [cif_mblist] *)
+  Lemma cif_mblist_unfold {α Φx l} :
+    cif_mblist α Φx l ≡ cif_mblist_gen α Φx (cif_mblist α Φx) l.
+  Proof. by rewrite /cif_mblist (profix_unfold (f:=cif_mblist_gen _ _) l). Qed.
+  (** Semantics *)
+  Definition mblist α Φx l : iProp Σ :=
+    mutex_bor α l (Φx (l +ₗ 1) ∗ ∃ l', ▷ (l +ₗ 2) ↦ #l' ∗ cif_mblist α Φx l').
+  (** Unfold semantics over [cif_ilist] *)
+  Lemma sem_mblist `{!NonExpansive δ} {α Φx l} :
+    cif_sem δ (cif_mblist α Φx l) ⊣⊢ mblist α Φx l.
+  Proof. by rewrite cif_mblist_unfold !sem_ecustom /=. Qed.
 
-  (** Iterate over [mblist] *)
+  (** Iterate over [cif_mblist] *)
   Definition iter_mblist : val := rec: "self" "f" "k" "c" "l" :=
     if: !"c" ≤ #0 then #true else
       if: try_acquire_loop_mutex "k" "l" then
@@ -526,7 +540,7 @@ Section verify.
   Lemma twp_iter_mblist {α Φx c l q} {f : val} {k n : nat} :
     (∀ l', [[{ ⟦ Φx (l' +ₗ 1) ⟧ }]][inv_wsat ⟦⟧ ∗ pborrow_wsat bupd ⟦⟧]
         f #(l' +ₗ 1) [[{ RET #(); ⟦ Φx (l' +ₗ 1) ⟧ }]]) -∗
-    [[{ c ↦ #n ∗ ⟦ mblist α Φx l ⟧ ∗ q.[α] }]]
+    [[{ c ↦ #n ∗ mblist α Φx l ∗ q.[α] }]]
       [inv_wsat ⟦⟧ ∗ pborrow_wsat bupd ⟦⟧]
       iter_mblist f #k #c #l
     [[{ b, RET #b; (if b then c ↦ #0 else ∃ n', c ↦ #n') ∗ q.[α] }]].
@@ -534,20 +548,23 @@ Section verify.
     iIntros "#f" (Ψ) "!> (c↦ & #m & α) →Ψ".
     iInduction n as [|m] "IH" forall (l) "m"=>/=.
     { wp_rec. wp_load. wp_pures. iApply "→Ψ". by iFrame. }
-    rewrite to_of_cit. wp_rec. wp_load. wp_pures.
+    wp_rec. wp_load. wp_pures.
     wp_apply (mutex_bor_try_acquire_loop with "[$m $α //]").
     iIntros ([|])=>/=; last first.
     { iIntros "[_ α]". wp_pure. iModIntro. iApply "→Ψ". iFrame. }
     iIntros "[b α]". wp_pures.
-    iMod (nbor_tok_open (M:=bupd) with "α b") as "/=[o (Φx & %l' & ↦ & mtl)]".
-    rewrite mblist'_unfold /=. iDestruct "mtl" as "#mtl".
-    wp_apply ("f" with "Φx"). iIntros "Φx". wp_load. wp_pures.
+    iMod (nbor_tok_open (M:=bupd) with "α b") as "/=[o (Φx & %l' & >↦ & mtl)]".
+    rewrite sem_mblist. iDestruct "mtl" as "#mtl". wp_apply ("f" with "Φx").
+    iIntros "Φx". wp_load. wp_pures.
     iMod (nobor_tok_close (M:=bupd) with "o [Φx ↦]") as "[α b]"=>/=.
-    { iFrame. by rewrite mblist'_unfold. }
+    { iFrame. by rewrite sem_mblist. }
     wp_apply (mutex_bor_release with "[$b $α //]"). iIntros "α". wp_load.
     wp_store. have -> : (S m - 1)%Z = m by lia.
     iApply ("IH" with "c↦ α →Ψ mtl").
   Qed.
+
+  Context `{!Inv'Con CON, !IffJudg (cifO CON Σ) JUDG, !Inv'Sem JUDG CON Σ,
+    !IffJsem (cifO CON Σ) Σ JUDG}.
 
   (** ** On derivability *)
 
@@ -559,7 +576,8 @@ Section verify.
   (** Turn [inv_tok] into [inv'] *)
   Lemma inv_tok_inv' `{!Deriv ih δ} {N Px} : inv_tok N Px ⊢ inv' δ N Px.
   Proof.
-    iIntros "$". iApply Deriv_factor. iIntros. iModIntro. iSplit; by iIntros.
+    iIntros "$". iApply Deriv_factor. iIntros. rewrite sem_ejudg. iModIntro.
+    iSplit; by iIntros.
   Qed.
 
   (** Access using [invd] *)
@@ -568,7 +586,7 @@ Section verify.
       ⟦ Px ⟧ ∗ (⟦ Px ⟧ =[inv_wsat ⟦⟧]{E∖↑N,E}=∗ True).
   Proof.
     iIntros (?) "[%Qx[#PQ i]]". iDestruct (der_sound with "PQ") as "{PQ}PQ".
-    iMod (inv_tok_acc with "i") as "[Qx cl]"; [done|].
+    iMod (inv_tok_acc with "i") as "[Qx cl]"; [done|]. rewrite sem_ejudg /=.
     iDestruct ("PQ" with "Qx") as "$". iIntros "!> Px". iApply "cl".
     by iApply "PQ".
   Qed.
@@ -599,8 +617,8 @@ Section verify.
       ⟦ Px ⟧(δ') ∗-∗ ⟦ Qx ⟧(δ')) -∗
       inv' δ N Px -∗ inv' δ N Qx.
   Proof.
-    iIntros "#iff [%Rx[#? i]]". iExists Rx. iFrame "i".
-    iApply Deriv_map; [|done]. iIntros (????). rewrite /⟦⟧(_) /=.
+    iIntros "#iff [%Rx[PR i]]". iExists Rx. iFrame "i".
+    iApply Deriv_map; [|done]. iIntros (????). rewrite !sem_ejudg /=.
     iIntros "#[PR RP] !>". iSplit.
     - iIntros "Qx". iApply "PR". by iApply "iff".
     - iIntros "Rx". iApply "iff"; [done..|]. by iApply "RP".
@@ -627,8 +645,8 @@ Section verify.
   Local Lemma inv'_inv'_sep_comm' `{!Deriv ih δ} {N N' Px Qx} :
     inv' δ N (cif_inv' N' (Px ∗ Qx)) ⊢ inv' δ N (cif_inv' N' (Qx ∗ Px)).
   Proof.
-    iApply inv'_iff. iIntros "!> /=" (????). rewrite !to_of_cit inv'_sep_comm.
-    iApply bi.wand_iff_refl.
+    iApply inv'_iff. iIntros "!> /=" (????). rewrite !sem_ecustom /=.
+    rewrite inv'_sep_comm. iApply bi.wand_iff_refl.
   Qed.
   Lemma inv'_inv'_sep_comm `{!Deriv ih δ} {N N' Px Qx} :
     inv' δ N (cif_inv' N' (Px ∗ Qx)) ⊣⊢ inv' δ N (cif_inv' N' (Qx ∗ Px)).
@@ -636,8 +654,8 @@ Section verify.
   Local Lemma inv'_bor_lft' `{!Deriv ih δ} {N α β Px} :
     α ⊑□ β -∗ β ⊑□ α -∗ inv' δ N (cif_bor α Px) -∗ inv' δ N (cif_bor β Px).
   Proof.
-    iIntros "#? #?". iApply inv'_iff. iIntros "!>" (????). rewrite /⟦⟧(_) /=.
-    iSplit; by iApply nbor_tok_lft.
+    iIntros "#? #?". iApply inv'_iff. iIntros "!>" (????).
+    rewrite /= !sem_ecustom /=. iSplit; by iApply nbor_tok_lft.
   Qed.
   Lemma inv'_bor_lft `{!Deriv ih δ} {N α β Px} :
     α ⊑□ β -∗ β ⊑□ α -∗ inv' δ N (cif_bor α Px) ∗-∗ inv' δ N (cif_bor β Px).
